\documentclass[12pt]{article}

\parindent=.25in
\setlength{\oddsidemargin}{0pt}
\setlength{\textwidth}{440pt}
\setlength{\topmargin}{0in}

\usepackage{amsmath}
\usepackage{amsfonts}
\usepackage[dvips]{graphicx}
\usepackage{verbatim}
\usepackage{appendix}

\title{COMS E6998 Homework 2}
\author{Mengqi Zong $<mz2326@columbia.edu>$}

\begin{document}

\maketitle

\setlength{\parindent}{0in}

\section*{Question 1}

Initialization: Set $q^0(y|w_1)$ and $r^0(w_2|y)$ to some initial
values (e.g. random initial values). \\

Algorithm: For $t = 1...T$: \\

1. For $i = 1...n$, and $y = 1...K$, calculate

\begin{eqnarray*}
\delta(y|i)
= p(y|w^i_1, w^i_2; \underline {\theta}^{t-1})
= \frac {q^{t-1}(y|w^i_1) r(w^i_2|y)}
{\sum_y {q^{t-1}(y|w^i_1) r(w^i_2|y)}}
\end{eqnarray*}

2. Recalculate the parameters: \\

\begin{eqnarray*}
q^t(y|w_1) = \frac {\sum_{i:w^i_1 = w_1} \delta (y|i)}
{\sum^n_{i=1} [[w^i_1 = w_1]]} \\
r^t(w_2|y) = \frac {\sum_{i:w^i_2 = w_2} \delta (y|i)}
{\sum^n_{i=1} \delta (y|i)}
\end{eqnarray*}

\section*{Question 2}

{\bf Question 2(a)}

\begin{eqnarray*}
P(y_2 = 1, y_3 = 2, y_4 = 1 | x; \theta)
= \frac {\alpha[2,1] \times t(2,1) \times e(x_3,2) \times t(1,2) \times
  e(x_4|1) \times \beta[4,1]} {\sum_s \alpha[n,s]}
\end{eqnarray*}

Note that $n$ is the length of the sequence of x. \\

{\bf Question 2(b)}

\begin{eqnarray*}
P(y_2 = 1, y_5 = 1|x; \theta)
= \frac {\sum_{y_3} \sum_{y_4} \alpha[2,1] t(y_3, 1) e(x_3,y_3) t(y_4,
  y_3) e(x_4, y_4) t(1, y_4) e(x_5, 1) \beta[5, 1]}
{\sum_s \alpha[n, s]}
\end{eqnarray*}

Note that $n$ is the length of the sequence of x. \\

{\bf Question 2(c)} \\

Here is the modified definition of the forward and backward terms:

\begin{eqnarray*}
\alpha' [j,s] &=&
\max_{s_1...s_{j-1}} [t(s_1)e(x_1|s_1)(\prod^{j-1}_{k=2}
t(s_k|s_{k-1})e(x_k|s_k))t(s|s_{j-1})e(x_J|s)] \\
\beta'[j,s] &=&
\max_{s_{j+1}...s_m}[t(s_{j+1}|s) e(x_{j+1}|s_{j+1}) (\prod^m_{k=j+2}
t(s_k|s_{k-1}) e(x_k|s_k))]
\end{eqnarray*}

Here is the recursive method. For $j = 2...m$:

\begin{eqnarray*}
\alpha' [j,s] &=& \max_{s' \in \{1..k\}} (\alpha'[j-1, s'] \times t(s|s')
\times e(x_j|s)) \\
\beta' [j,s] &=& \max_{s' \in \{1..k\}} (\beta'[j+1, s'] \times t(s'|s)
\times e(x_{j+1}|s'))
\end{eqnarray*}

The probability we want to calculate is:

\begin{eqnarray*}
\max_{y:y_j = p} p(y|x; \theta)
&=& \alpha'[j,p] \times \beta'[j,p] \\
\max_{y:y_3 = 1} p(y|x; \theta)
&=& \alpha'[3,1] \times \beta'[3,1]
\end{eqnarray*}

\section*{Question 3}

{\bf Question 3(a)}

\begin{eqnarray*}
\alpha [j,a] &=& \sum_{a_1...a_{j-1}} [d(a_1|a_0)t(f_1|e_{a_1}))
(\prod^{j-1}_{k=2} d(a_k|a_{k-1}) t(f_k|e_{a_k}))
d(a|a_{j-1})t(f_j|e_{a_j})] \\
\beta [j,a] &=& \sum_{a_{j+1}...a_m}
[d(a_{j+1}|a)e(f_{j+1}|e_{a_{j+1}}) (\prod^m_{k=j+2}
d(a_k|a_{k-1})e(f_k|e_{a_k}))]
\end{eqnarray*}

Then we have

\begin{equation*}
P(a_j=k|f,e) = \alpha [j,k] \times \beta [j,k]
\end{equation*}

{\bf Question 3(b)}

\begin{eqnarray*}
P(a_j = k, a_{j+1} = k'|f,e) = \alpha [j, k] \times d(k'|k) \times
t(f_{j+1}|e_{k'}) \times \beta [j+1, k']
\end{eqnarray*}

{\bf Question 3(c)} \\

Define $\overline {count}(i, a \to a'; \underline {\theta})$ to be
the expected number of times the transition  $a \to a'$ is seen
in the training example $f^{(i)}, e^{(i)}$, for parameters $\underline
{\theta}$. Then

\begin{eqnarray*}
\overline {count}(i, a \to a'; \underline {\theta}) =
\sum^{m-1}_{j=1} p(a_j = a, a_{j+1} = a'| f^{(i)}, e^{(i)}; \underline
{\theta})
\end{eqnarray*}

Define $\overline {count}(i, e \rightsquigarrow f; \underline
{\theta})$ to be the expected number of times the English word $e$ is
paired with the French word $f$ in the training example $f^{(i)},
e^{(i)}$, for parameters $\underline {\theta}$. Then

\begin{eqnarray*}
\overline {count}(i, e \rightsquigarrow f; \underline {\theta}) =
\sum^{m-1}_{j=1} p(a_j = a_e | f^{(i)}, e^{(i)}; \underline {\theta})
\end{eqnarray*}

The EM algorithm:

\begin{itemize}
\item Initialization: set initial parameters $\underline {\theta}^0$ to
  some value
\item For $t = 1...T$:
  \begin{itemize}
  \item Use the forward-backward algorithm to compute all expected
    counts of the form
    \begin{eqnarray*}
      \overline {count}(i, a \to a'; \underline {\theta}^{t-1})
      \text{ or }
      \overline {count}(i, e \rightsquigarrow f; \underline
      {\theta}^{t-1})
    \end{eqnarray*}
  \item Update the parameters based on the expected counts:
    \begin{eqnarray*}
      d^t(a'|a) = \frac {\sum^n_{i=1} \overline {count}(i, a \to a';
        \underline {\theta}^{t-1})}
      {\sum^n_{i=1} \sum_{a'} \overline {count}(i, a \to a';
        \underline {\theta}^{t-1})} \\
      t^t(f|e) = \frac {\sum^n_{i=1} \overline {count}(i, e
        \rightsquigarrow f; \underline {\theta}^{t-1})}
      {\sum^n_{i=1} \sum_f \overline {count}(i, e \rightsquigarrow f;
        \underline {\theta}^{t-1})}
    \end{eqnarray*}
  \end{itemize}
\end{itemize}

\end{document}
